working in the simulation relation of the example with mutual recursion. Define an inductive prop to describe the continuation frame

demo/ClientServerMRCSpec.v
@@ -21,11 +21,10 @@ Definition input_index_def_unit :=
     gvar_readonly := false;
     gvar_volatile := false |}.
 
-Compute (link (skel (Clight.semantics1 client)) (skel L2)).
 
-Definition linked_skel2 : program unit unit:=
+Definition linked_skel1 : program unit unit:=
   {|
-    prog_defs := (result_id, Gvar result_def_unit) :: (key_id, Gvar key_def_const) ::
+    prog_defs := (result_id, Gvar result_def_unit) :: (key_id, Gvar key_def) ::
                    (input_id, Gvar input_index_def_unit) ::
                    (encrypt_id, Gfun tt) :: (request_id, Gfun tt) ::
                    (index_id, Gvar input_index_def_unit) :: nil;
@@ -34,18 +33,297 @@ Definition linked_skel2 : program unit unit:=
     prog_main := 42%positive
   |}.
 
-Compute linked_skel2.
+Section WITH_N.
 
-Theorem link_ok2 :
-  link (skel (Clight.semantics1 client)) (skel L2) = Some linked_skel2.
+Variable N: Z.  
+
+Let client := client N.
+Let func_request := func_request N.
+
+Theorem link_ok1 :
+  link (skel (Clight.semantics1 client)) (skel L1) = Some linked_skel1.
 Proof. reflexivity. Qed.
 
-Definition L := fun i : bool => if i then (Clight.semantics1 client) else L2.
-Definition composed_spec2 := semantics L linked_skel2.
+Definition L := fun i : bool => if i then (Clight.semantics1 client) else L1.
+Definition composed_spec1 := semantics L linked_skel1.
 
 Theorem link_result :
-  compose (Clight.semantics1 client) L2 = Some composed_spec2.
+  compose (Clight.semantics1 client) L1 = Some composed_spec1.
 Proof.
-  unfold compose. rewrite link_ok2. simpl. reflexivity.
+  unfold compose. rewrite link_ok1. simpl. reflexivity.
 Qed.
 
+
+(** * C-level top specification *)
+
+Inductive state : Type :=
+| Callrequest (input : int) (m:mem)
+| Callencrypt (input : int) (fptr : val) (m:mem)
+| Return (m:mem).
+
+Definition genv := Genv.t unit unit.
+
+Section WITH_SE.
+Context (se:Genv.symtbl).
+
+Inductive initial_state : query li_c ->  state -> Prop :=
+|initial_request output m fb
+   (FIND: Genv.find_symbol se request_id = Some fb):
+  initial_state (cq (Vptr fb Ptrofs.zero) int__void_sg ((Vint output) :: nil) m)
+    (Callrequest output m)
+|initial_encrypt i fb b ofs m
+   (FIND: Genv.find_symbol se encrypt_id = Some fb):
+  initial_state (cq (Vptr fb Ptrofs.zero) int_fptr__void_sg ((Vint i) :: (Vptr b ofs) :: nil) m)
+    (Callencrypt i (Vptr b ofs) m).
+
+Inductive at_external : state -> query li_c -> Prop :=.
+Inductive after_external : state -> c_reply -> state -> Prop := .
+
+Inductive final_state : state -> reply li_c -> Prop :=
+|final_process m:
+  final_state (Return m) (cr Vundef m).
+
+Definition valid_query (q: query li_c) : bool :=
+  match (cq_vf q) with
+  |Vptr b ofs =>  if Ptrofs.eq_dec ofs Ptrofs.zero then
+                  match Genv.invert_symbol se b with
+                  | Some 3%positive | Some  1%positive => true
+                  | _ => false
+                  end
+                  else false
+  |_  => false
+  end.
+
+Definition Nint := (Int.repr N).
+
+Inductive step : state -> trace -> state -> Prop :=
+| step_request1 r input rb idb inb idx m m'
+  (FINDIDX: Genv.find_symbol se index_id = Some idb)
+  (FINDREQ: Genv.find_symbol se request_id = Some rb)
+  (FINDINPUT: Genv.find_symbol se input_id = Some inb)
+  (READIDX: Mem.loadv Mint32 m (Vptr idb Ptrofs.zero) = Some (Vint idx))
+  (COND: Int.eq idx Int.zero = true)
+  (ADDIDX: Mem.storev Mint32 m (Vptr idb Ptrofs.zero) (Vint (Int.add idx Int.one)) = Some m')
+  (READINPUT: Mem.loadv Mint32 m' (Vptr inb (Ptrofs.sub (Ptrofs.of_int idx) (Ptrofs.one))) = Some (Vint input)):
+  step (Callrequest r m) E0 (Callencrypt input (Vptr rb Ptrofs.zero) m')
+| step_request2 r input rb idb inb rsb idx m m' m''
+  (FINDIDX: Genv.find_symbol se index_id = Some idb)
+  (FINDREQ: Genv.find_symbol se request_id = Some rb)
+  (FINDINPUT: Genv.find_symbol se input_id = Some inb)
+  (FINDRES: Genv.find_symbol se result_id = Some rsb)
+  (READIDX: Mem.loadv Mint32 m (Vptr idb Ptrofs.zero) = Some (Vint idx))
+  (COND: Int.lt Int.zero idx && Int.lt idx Nint = true)
+  (STORERES: Mem.storev Mint32 m (Vptr rsb (Ptrofs.sub (Ptrofs.of_int idx) (Ptrofs.one))) (Vint r) = Some m')
+  (ADDIDX: Mem.storev Mint32 m' (Vptr idb Ptrofs.zero) (Vint (Int.add idx Int.one)) = Some m'')
+  (READINPUT: Mem.loadv Mint32 m'' (Vptr inb (Ptrofs.sub (Ptrofs.of_int idx) (Ptrofs.one))) = Some (Vint input)):
+  step (Callrequest r m) E0 (Callencrypt input (Vptr rb Ptrofs.zero) m'')
+| step_request3 r idb rsb idx m m'
+  (FINDIDX: Genv.find_symbol se index_id = Some idb)
+  (FINDRES: Genv.find_symbol se result_id = Some rsb)
+  (READIDX: Mem.loadv Mint32 m (Vptr idb Ptrofs.zero) = Some (Vint idx))
+  (COND: Int.cmp Cge idx Nint = true)
+  (STORERES: Mem.storev Mint32 m (Vptr rsb (Ptrofs.sub (Ptrofs.of_int idx) (Ptrofs.one))) (Vint r) = Some m'):
+  step (Callrequest r m) E0 (Return m')
+| step_encrypt kb rb key input m output
+   (FINDK: Genv.find_symbol se key_id = Some kb)
+   (FINDP: Genv.find_symbol se request_id = Some rb)
+   (READ: Mem.loadv Mint32 m (Vptr kb Ptrofs.zero) = Some (Vint key))
+   (XOR: output = Int.xor input key):
+  step (Callencrypt input (Vptr rb Ptrofs.zero) m) E0 (Callrequest output m).
+
+End WITH_SE.
+
+Program Definition top_spec1 : Smallstep.semantics li_c li_c :=
+    {|
+      Smallstep.skel := linked_skel1;
+      Smallstep.state := state;
+      Smallstep.activate se :=
+        {|
+          Smallstep.step _ := step se;
+          Smallstep.valid_query := valid_query se;
+          Smallstep.initial_state := initial_state se;
+          Smallstep.at_external := at_external;
+          Smallstep.after_external := after_external;
+          Smallstep.final_state := final_state;
+          globalenv := tt;
+        |}
+    |}.
+
+(** Proof of top_spec -> composed_spec1 *)
+
+Section MS.
+
+Variable w: injp_world.
+Variable se tse : Genv.symtbl.
+
+Let tge1 := Clight.globalenv tse client.
+Let tge2 := Genv.globalenv tse b1.
+
+Hypothesis MSTB : match_stbls injp w se tse.
+
+Inductive match_kframe_request : list (frame L) -> Prop :=
+| match_kframe_request_nil:
+  match_kframe_request nil
+| match_kframe_request_call2 output m fb:
+  match_kframe_request ((st L false (Call2 fb output m)) :: nil)
+| match_kframe_request_cons output m fb1 fb2 vargs k sp le:
+  match_kframe_request k ->
+  match_kframe_request ((st L false (Call2 fb1 output m)) :: (st L true (Callstate fb2 vargs (Kcall None func_request (Maps.PTree.set r_id (sp, Ctypesdefs.tint) empty_env) le Kstop) m)) :: k).
+
+Inductive match_kframe_encrypt : list (frame L) -> Prop :=
+| match_kframe_encrypt_nil:
+  match_kframe_encrypt nil
+| match_kframe_encrypt_callstate m fb sp le vargs:
+  match_kframe_encrypt ((st L true (Callstate fb vargs (Kcall None func_request (Maps.PTree.set r_id (sp, Ctypesdefs.tint) empty_env) le Kstop) m)) :: nil)
+| match_kframe_encrypt_cons output m fb1 fb2 vargs k sp le:
+  match_kframe_encrypt k ->
+  match_kframe_encrypt ((st L true (Callstate fb2 vargs (Kcall None func_request (Maps.PTree.set r_id (sp, Ctypesdefs.tint) empty_env) le Kstop) m)) :: (st L false (Call2 fb1 output m)) :: k).
+
+
+Inductive match_state: state -> list (frame L) -> Prop :=
+| match_request_intro j r rb rb' m tm ks
+    (Hm: Mem.inject j m tm)
+    (INJP: injp_acc w (injpw j m tm Hm))
+    (FINDP: Genv.find_symbol se request_id = Some rb)
+    (FINJ: j rb = Some (rb',0))
+    (KFRM: match_kframe_request ks):
+  match_state (Callrequest r m) ((st L true (Callstate (Vptr rb' Ptrofs.zero) (Vint r :: nil) Kstop tm)) :: ks)
+| match_encrypt_intro j v tv m tm input ks
+    (Hm: Mem.inject j m tm)
+    (INJP: injp_acc w (injpw j m tm Hm))
+    (VINJ: Val.inject j v tv)
+    (KFRM: match_kframe_encrypt ks):
+  match_state (Callencrypt input v m) ((st L false (Call1 tv input tm)) :: ks)
+| match_return_introc j m tm
+  (Hm: Mem.inject j m tm)
+  (INJP : injp_acc w (injpw j m tm Hm)):
+  match_state (Return m) (st L true (Returnstate Vundef Kstop tm) :: nil)
+|match_return_intros j m tm
+  (Hm: Mem.inject j m tm)
+  (INJP : injp_acc w (injpw j m tm Hm)):
+  match_state (Return m) ((st L false (Return2 tm)) :: nil).
+
+Lemma find_request:
+  forall rb rb' j,
+    Genv.match_stbls j se tse ->
+    Genv.find_symbol se request_id = Some rb ->
+    j rb = Some (rb',0) ->
+    Genv.find_funct tge1 (Vptr rb' Ptrofs.zero) = Some (Ctypes.Internal func_request).
+Proof.
+Admitted.
+
+Lemma find_encrypt:
+  forall rb rb' j,
+    Genv.match_stbls j se tse ->
+    Genv.find_symbol se encrypt_id = Some rb ->
+    j rb = Some (rb',0) ->
+    Genv.find_funct tge2 (Vptr rb' Ptrofs.zero) = Some (Internal func_encrypt_b1).
+Proof.
+Admitted.
+
+
+End MS.
+
+Lemma top_simulation_L1:
+  forward_simulation (cc_c injp) (cc_c injp) top_spec1 composed_spec1.
+Proof.
+  constructor. econstructor; eauto. instantiate (1 := fun _ _ _ => _). cbn beta.
+  intros se1 se2 w Hse Hse1. cbn in *. subst.
+  pose (ms := fun s1 s2 => match_state w se1 s1 s2).
+  eapply forward_simulation_plus with (match_states := ms).
+  destruct w as [f0 m0 tm0 Hm0]; cbn in Hse; inv Hse; subst; cbn in *; eauto.
+  - intros. inv H. cbn in *. inv H3.
+    unfold valid_query.
+    unfold L. simpl.
+    unfold SmallstepLinking.valid_query, Smallstep.valid_query.
+    simpl. inv H0;try congruence; simpl; eauto.
+    destruct (Genv.invert_symbol se1 b1) eqn:INV.
+    2: {
+      unfold Genv.is_internal, Genv.find_funct, Genv.find_funct_ptr.
+      rewrite !Genv.find_def_spec.
+      assert (Genv.invert_symbol se2 b2 = None).
+      destruct (Genv.invert_symbol se2 b2) as [i|] eqn:FIND2; eauto.
+      apply Genv.invert_find_symbol in FIND2.
+      inv H2.
+      eapply mge_symb in FIND2 as FIND1; eauto.
+      apply Genv.find_invert_symbol in FIND1. congruence.
+      rewrite H0.
+      destruct Ptrofs.eq_dec; destruct Ptrofs.eq_dec; eauto.
+    }
+        apply Genv.invert_find_symbol in INV as FIND.
+    assert (delta = 0).
+    { inv H2. exploit mge_dom. eapply Genv.genv_symb_range; eauto.
+      intros [a b]. rewrite H in b. inv b. reflexivity.
+    }
+    subst delta.
+    destruct (Ptrofs.eq_dec ofs1 Ptrofs.zero).
+    2: {
+      unfold Genv.is_internal. unfold Genv.find_funct.
+      rewrite !pred_dec_false. reflexivity.
+      rewrite Ptrofs.add_zero. auto.
+      rewrite Ptrofs.add_zero. auto.
+    }
+    unfold Genv.is_internal.
+    rewrite !Ptrofs.add_zero. subst ofs1.
+    destruct (peq i 3).
+   + subst. setoid_rewrite find_request;eauto. cbn. econstructor;eauto.
+   + destruct (peq i 1).
+      ++ subst i. setoid_rewrite find_encrypt; eauto.
+         destruct (Genv.find_funct); cbn; eauto.
+         destruct fundef_is_internal; reflexivity.
+         cbn. econstructor;eauto.
+      ++ admit.
+         
+  - intros q1 q2 s1 Hq Hi1. inv Hq. inv H1. inv Hi1; cbn in *.
+    + (* initial request *)
+      inv Hse.
+      eapply Genv.find_symbol_match in H5 as FIND'; eauto.
+      destruct FIND' as [fb' [FINJ FIND']]. inv H.
+      inv H0. inv H7. inv H3.
+      rewrite FINJ in H4. inv H4. rename b2 into fb'. rewrite Ptrofs.add_zero.
+      exploit find_request; eauto.  cbn; econstructor;eauto. intro FINDR.
+      exists ((st L true (Callstate (Vptr fb' Ptrofs.zero) (Vint output :: nil) Kstop m2)) :: nil).
+      split. split.
+      -- simpl. unfold Genv.is_internal. setoid_rewrite FINDR. reflexivity.
+      -- simpl.
+       set (targs := (Ctypes.Tcons
+            (Ctypes.Tint Ctypes.I32 Ctypes.Signed
+                         {| Ctypes.attr_volatile := false; Ctypes.attr_alignas := None |}) Ctypes.Tnil)).
+       assert (Ctypes.signature_of_type targs Ctypes.Tvoid cc_default = int__void_sg).
+       reflexivity.
+       rewrite <- H.
+       econstructor; eauto.
+       constructor; cbn; eauto. constructor; eauto. constructor.
+      -- econstructor; eauto. reflexivity. constructor.
+    + (* initial encrypt *)
+            inv Hse.
+      eapply Genv.find_symbol_match in H5 as FIND'; eauto.
+      destruct FIND' as [fb' [FINJ FIND']]. inv H.
+      inv H0. inv H7. inv H3. inv H10.
+      rewrite FINJ in H4. inv H4. rename b2 into fb'. rewrite Ptrofs.add_zero.
+      exploit find_encrypt; eauto. cbn;econstructor;eauto. intro FINDE.
+      exists ((st L false (Call1 v'0 i m2)) :: nil).
+      split. split.
+      -- simpl. unfold Genv.is_internal.
+         setoid_rewrite find_encrypt; eauto.
+         cbn;econstructor;eauto.
+      -- simpl. inv H1. econstructor; eauto.
+      -- inv H1.
+         econstructor;eauto. reflexivity.
+         constructor.
+  (* final state *)
+  - intros s1 s2 r1 Hms Hf1. inv Hf1. inv Hms;
+      try inv H; cbn in *.
+    +  exists (cr Vundef tm). split. cbn.
+       constructor. constructor.
+       eexists. split. eauto. constructor; eauto. constructor.
+    + (*final of server*)
+      exists (cr Vundef tm). split. cbn.
+      constructor. constructor.
+      eexists. split. eauto. constructor; eauto. constructor.
+  - intros. cbn in *. inv H0.
+  (* step *)
+  - Admitted.
+        
+End MS.
+End WITH_N.
